code/experimental/P256/testECDSAVerification.c
@@ -1,0 +1,235 @@
+#include <inttypes.h>
+#include <stdio.h>
+#include <stdlib.h>
+#include <string.h>
+#include <sys/types.h>
+#include <sys/stat.h>
+#include <fcntl.h>
+#include <unistd.h>
+#include <stdbool.h>
+#include <time.h>
+
+
+#include "ecdsap256-c/Hacl_Impl_ECDSA_P256SHA256_Verification.h"
+
+#include <stdio.h>
+#include <stdlib.h>
+
+#include <unistd.h>
+
+
+typedef __attribute__((aligned(32))) uint8_t POINT[12 * 8];
+typedef __attribute__((aligned(32))) uint8_t SCALAR[32];
+
+typedef uint64_t cycles;
+
+static __inline__ cycles cpucycles(void)
+{
+  uint64_t rax,rdx,aux;
+  asm volatile ( "rdtscp\n" : "=a" (rax), "=d" (rdx), "=c" (aux) : : );
+  return (rdx << 32) + rax;
+}
+#define ROUNDS 10000
+#define SIZE   1
+
+uint64_t generateRandom()
+{
+   return (uint64_t) (((uint64_t) rand() << 33) | rand())%18446744073709551615U;
+}
+
+
+void print_u(uint64_t a)
+{
+   printf("%" PRIu64 " ", a);
+   printf("%u ", (uint32_t) a);
+   printf("%u\n", (uint32_t) (a >> 32));
+}
+
+void print_uu(uint64_t* a)
+{
+   print_u(a[0]);
+   print_u(a[1]);
+   print_u(a[2]);
+   print_u(a[3]);
+   printf("\n");
+}
+
+void printfb(bool result)
+{
+  if (result == 0)
+    printf("%s\n", "false");
+  else if (result == 1)
+    printf("%s\n", "true");
+  else
+    printf("%s\n", "magic");  
+}
+
+void test1()
+   {
+      uint8_t* m = (uint8_t *) malloc (sizeof (uint8_t) * 128);
+     m[0] = 0xe1;
+m[1] = 0x13;
+m[2] = 0x0a;
+m[3] = 0xf6;
+m[4] = 0xa3;
+m[5] = 0x8c;
+m[6] = 0xcb;
+m[7] = 0x41;
+m[8] = 0x2a;
+m[9] = 0x9c;
+m[10] = 0x8d;
+m[11] = 0x13;
+m[12] = 0xe1;
+m[13] = 0x5d;
+m[14] = 0xbf;
+m[15] = 0xc9;
+m[16] = 0xe6;
+m[17] = 0x9a;
+m[18] = 0x16;
+m[19] = 0x38;
+m[20] = 0x5a;
+m[21] = 0xf3;
+m[22] = 0xc3;
+m[23] = 0xf1;
+m[24] = 0xe5;
+m[25] = 0xda;
+m[26] = 0x95;
+m[27] = 0x4f;
+m[28] = 0xd5;
+m[29] = 0xe7;
+m[30] = 0xc4;
+m[31] = 0x5f;
+m[32] = 0xd7;
+m[33] = 0x5e;
+m[34] = 0x2b;
+m[35] = 0x8c;
+m[36] = 0x36;
+m[37] = 0x69;
+m[38] = 0x92;
+m[39] = 0x28;
+m[40] = 0xe9;
+m[41] = 0x28;
+m[42] = 0x40;
+m[43] = 0xc0;
+m[44] = 0x56;
+m[45] = 0x2f;
+m[46] = 0xbf;
+m[47] = 0x37;
+m[48] = 0x72;
+m[49] = 0xf0;
+m[50] = 0x7e;
+m[51] = 0x17;
+m[52] = 0xf1;
+m[53] = 0xad;
+m[54] = 0xd5;
+m[55] = 0x65;
+m[56] = 0x88;
+m[57] = 0xdd;
+m[58] = 0x45;
+m[59] = 0xf7;
+m[60] = 0x45;
+m[61] = 0x0e;
+m[62] = 0x12;
+m[63] = 0x17;
+m[64] = 0xad;
+m[65] = 0x23;
+m[66] = 0x99;
+m[67] = 0x22;
+m[68] = 0xdd;
+m[69] = 0x9c;
+m[70] = 0x32;
+m[71] = 0x69;
+m[72] = 0x5d;
+m[73] = 0xc7;
+m[74] = 0x1f;
+m[75] = 0xf2;
+m[76] = 0x42;
+m[77] = 0x4c;
+m[78] = 0xa0;
+m[79] = 0xde;
+m[80] = 0xc1;
+m[81] = 0x32;
+m[82] = 0x1a;
+m[83] = 0xa4;
+m[84] = 0x70;
+m[85] = 0x64;
+m[86] = 0xa0;
+m[87] = 0x44;
+m[88] = 0xb7;
+m[89] = 0xfe;
+m[90] = 0x3c;
+m[91] = 0x2b;
+m[92] = 0x97;
+m[93] = 0xd0;
+m[94] = 0x3c;
+m[95] = 0xe4;
+m[96] = 0x70;
+m[97] = 0xa5;
+m[98] = 0x92;
+m[99] = 0x30;
+m[100] = 0x4c;
+m[101] = 0x5e;
+m[102] = 0xf2;
+m[103] = 0x1e;
+m[104] = 0xed;
+m[105] = 0x9f;
+m[106] = 0x93;
+m[107] = 0xda;
+m[108] = 0x56;
+m[109] = 0xbb;
+m[110] = 0x23;
+m[111] = 0x2d;
+m[112] = 0x1e;
+m[113] = 0xeb;
+m[114] = 0x00;
+m[115] = 0x35;
+m[116] = 0xf9;
+m[117] = 0xbf;
+m[118] = 0x0d;
+m[119] = 0xfa;
+m[120] = 0xfd;
+m[121] = 0xcc;
+m[122] = 0x46;
+m[123] = 0x06;
+m[124] = 0x27;
+m[125] = 0x2b;
+m[126] = 0x20;
+m[127] = 0xa3;
+
+
+      uint32_t mLen = 128;
+      uint64_t* pubKey = (uint64_t *) malloc (sizeof (uint64_t) * 12);
+      uint64_t* r = (uint64_t *) malloc (sizeof (uint64_t) * 4);
+      uint64_t* s = (uint64_t *) malloc (sizeof (uint64_t) * 4);
+      
+      pubKey[3] = 0xe424dc61d4bb3cb7ul;
+      pubKey[2] = 0xef4344a7f8957a0cul;
+      pubKey[1] = 0x5134e16f7a67c074ul;
+      pubKey[0] = 0xf82e6e12f49abf3cul;
+
+      pubKey[7] = 0x970eed7aa2bc4865ul;
+      pubKey[6] = 0x1545949de1dddaf0ul;
+      pubKey[5] = 0x127e5965ac85d124ul;
+      pubKey[4] = 0x3d6f60e7dfaee927ul;
+
+      r[3] =  0xbf96b99aa49c705cul;
+      r[2] =  0x910be33142017c64ul;
+      r[1] =  0x2ff540c76349b9daul;
+      r[0] =  0xb72f981fd9347f4ful;
+ 
+      s[3] =  0x17c55095819089c2ul;
+      s[2] =  0xe03b9cd415abdf12ul;
+      s[1] =  0x444e323075d98f31ul;
+      s[0] =  0x920b9e0f57ec871cul;
+
+      bool result = Hacl_Impl_ECDSA_P256SHA256_Verification_ecdsa_verification (pubKey, r, s, mLen, m);
+      printfb(result);
+
+
+   }
+
+int main()
+{
+   test1();
+
+}
