code/experimental/P256/Hacl.Impl.P256.fsti
@@ -118,6 +118,16 @@ val point_add: p: point -> q: point -> result: point -> tempBuffer: lbuffer uint
   )
 
 
+val toJ: p: point -> resultPoint: point -> tempBuffer: lbuffer uint64 (size 88) -> Stack unit
+  (requires fun h -> live h p /\ live h resultPoint /\ live h tempBuffer /\ disjoint p tempBuffer /\ disjoint tempBuffer resultPoint /\ 
+    as_nat h (gsub p (size 0) (size 4)) < prime /\
+    as_nat h (gsub p (size 4) (size 4)) < prime /\
+    as_nat h (gsub p (size 8) (size 4)) < prime 
+  ) 
+  (ensures fun h0 _ h1 -> True  )
+
+
+
 val norm: p: point -> resultPoint: point -> tempBuffer: lbuffer uint64 (size 88) -> Stack unit
   (requires fun h -> live h p /\ live h resultPoint /\ live h tempBuffer /\ disjoint p tempBuffer /\ disjoint tempBuffer resultPoint /\ 
     as_nat h (gsub p (size 0) (size 4)) < prime /\
@@ -171,7 +181,30 @@ val scalarMultiplication: #buf_type: buftype->  p: point -> result: point ->
 ) 
 
 
-val secretToPublic: result: point -> scalar: lbuffer uint8 (size 32) -> 
+val scalarMultiplicationWithoutNorm: p: point -> result: point -> 
+  scalar: lbuffer  uint8 (size 32) -> 
+  tempBuffer: lbuffer uint64 (size 100) ->
+  Stack unit
+    (requires fun h -> 
+      live h p /\ live h result /\ live h scalar /\ live h tempBuffer /\
+    LowStar.Monotonic.Buffer.all_disjoint [loc p; loc tempBuffer; loc scalar; loc result] /\
+    as_nat h (gsub p (size 0) (size 4)) < prime /\ 
+    as_nat h (gsub p (size 4) (size 4)) < prime /\
+    as_nat h (gsub p (size 8) (size 4)) < prime
+    )
+  (ensures fun h0 _ h1 -> 
+    modifies3 p result tempBuffer h0 h1 /\ 
+    modifies (loc p |+| loc result |+| loc tempBuffer) h0 h1 /\
+    (
+      let x3, y3, z3 = point_x_as_nat h1 result, point_y_as_nat h1 result, point_z_as_nat h1 result in 
+      let (xN, yN, zN) = scalar_multiplication (as_seq h0 scalar) (point_prime_to_coordinates (as_seq h0 p)) in 
+      x3 == xN /\ y3 == yN /\ z3 == zN 
+  )
+) 
+
+
+
+val secretToPublicWithoutNorm: result: point -> scalar: lbuffer uint8 (size 32) -> 
  tempBuffer: lbuffer uint64 (size 100) ->
   Stack unit
     (requires fun h -> 
